pulse/examples/steel/AggregateRef.fsti
@@ -227,24 +227,120 @@ let mpts_to (#p: pcm 'a) (r: Steel.Memory.ref 'a p) = Steel.PCMReference.pts_to 
 let pts_to (r: ref 'a 'b) (v: Ghost.erased 'b): vprop = (* TODO unerase v, try [@@@smt_fallback] *)
   r.r `mpts_to` put r.pl v (one (refined_pcm r.re))
 
-(** A pcm_lens for the k-th field of an n-ary product *)
-val field (#a:eqtype) (#b:a -> Type) (p:(k:a -> pcm (b k))) (k:a): pcm_lens (prod_pcm p) (p k)
+(** A lens for the k-th field of an n-ary product *)
+
+let fun_upd (#a:eqtype) #f_ty (k:a) (x':f_ty k)
+  (f: restricted_t a f_ty)
+: restricted_t a f_ty
+= on_domain a (fun k' -> if k = k' then x' else f k')
+let lens_field_get (#a:eqtype) f (k:a) (s:restricted_t a f): f k = s k
+let lens_field (#a:eqtype) f (k:a): lens (restricted_t a f) (f k) = {
+  get = lens_field_get f k;
+  put = fun_upd k;
+  get_put = (fun s v -> ());
+  put_get = (fun s -> ext (fun_upd k (lens_field_get f k s) s) s (fun _ -> ()));
+  put_put = (fun s v w -> ext (fun_upd k v (fun_upd k w s)) (fun_upd k v s) (fun _ -> ()));
+}
+
+(** lens_field is a pcm_lens *)
+
+(* TODO move to Aggregates.fst *)
+let prod_pcm_composable_intro (p:(k:'a -> pcm ('b k))) (x y: restricted_t 'a 'b)
+  (h:(k:'a -> Lemma (composable (p k) (x k) (y k))))
+: Lemma (composable (prod_pcm p) x y) = FStar.Classical.forall_intro h
+
+let field (#a:eqtype) #f (p:(k:a -> pcm (f k))) (k:a): pcm_lens (prod_pcm p) (p k) = {
+  l = lens_field f k;
+  get_morphism = {f_refine = (fun _ -> ()); f_one = (fun _ -> ()); f_op = (fun _ _ -> ())};
+  put_morphism = {
+    f_refine = (fun _ -> ());
+    f_one = (fun _ ->
+      ext
+        (fun_upd k (one (p k)) (one (prod_pcm p)))
+        (one (prod_pcm p))
+        (fun k -> ()));
+    f_op = (fun (v, s) (w, t) ->
+      prod_pcm_composable_intro p (fun_upd k v s) (fun_upd k w t) (fun _ -> ());
+      ext
+        (fun_upd k (op (p k) v w) (op (prod_pcm p) s t))
+        (op (prod_pcm p) (fun_upd k v s) (fun_upd k w t))
+        (fun _ -> ()));
+  }
+}
 
 (** The refinement of an n-ary union PCM to the k-th case *)
 
-val case_refinement
-  (#b:'a -> Type)
-  (p:(k:'a -> refined_one_pcm (b k))) (k:'a)
-: pcm_refinement (union_pcm p)
+let case_refinement_f (p:(k:'a -> pcm ('b k))) (k:'a): union 'b -> prop =
+  fun kx -> match kx with Some (|k', _|) -> k == k' | None -> False
 
-val case_unrefinement
-  (#a:eqtype) (#b:a -> Type)
-  (p:(k:a -> refined_one_pcm (b k))) (k:a)
+let case_refinement_new_one (p:(k:'a -> pcm ('b k))) (k:'a)
+: refine_t (case_refinement_f p k)
+= Some (|k, one (p k)|)
+
+let case_refinement (p:(k:'a -> refined_one_pcm ('b k))) (k:'a)
+: pcm_refinement (union_pcm p) = {
+  f = case_refinement_f p k;
+  f_closed_comp = (fun x y -> ());
+  new_one = case_refinement_new_one p k;
+  new_one_is_refined_unit = (fun (Some (|k', x|)) -> (p k).is_unit x)
+}
+
+(* TODO could be made abstract? *)
+let case_unrefinement (#a:eqtype) #b (p:(k:a -> refined_one_pcm (b k))) (k:a)
 : pcm_unrefinement (case_refinement p k)
+= fun kx ky f kv ->
+  let p' = refined_pcm (case_refinement p k) in
+  let p = union_pcm p in
+  match kv with
+  | Some (|k', v|) ->
+    if k = k' then begin
+      let _ = Ghost.hide (
+        let Some (|k, x|) = Ghost.reveal kx in
+        let goal = compatible p' kx kv in
+        compatible_elim p kx kv goal (fun kx_frame -> match kx_frame with
+          | Some (|_, frame_x|) -> compatible_intro p' kx kv (Some (|k, frame_x|))
+          | None -> compatible_refl p' kx))
+      in
+      let kw = f kv in
+      let aux (frame:union b{composable p kx frame})
+      : Lemma (composable p ky frame /\
+               (op p kx frame == Some (|k, v|) ==>
+                op p ky frame == f (Some (|k, v|))))
+      = let Some (|_, w|) = f (Some (|k, v|)) in
+        match frame with
+        | Some (|frame_k, frame_v|) -> assert (composable p' kx frame)
+        | None ->
+          p'.is_unit kx;
+          assert (composable p' kx (one p'));
+          p'.is_unit ky
+      in FStar.Classical.forall_intro aux;
+      kw
+    end else None
+  | _ -> None
 
-(** A pcm_lens for the k-th case of an n-ary union *)
-val case (#b:'a -> Type) (p:(k:'a -> refined_one_pcm (b k))) (k:'a)
-: pcm_lens (refined_pcm (case_refinement p k)) (p k)
+(** A lens for the k-th case of an n-ary union *)
+
+let lens_case_get (p:(k:'a -> pcm ('b k))) (k:'a): refine_t (case_refinement_f p k) -> 'b k =
+  fun (Some (|_, v|)) -> v
+let lens_case_put (p:(k:'a -> pcm ('b k))) (k:'a) (v:'b k)
+: refine_t (case_refinement_f p k) -> refine_t (case_refinement_f p k)
+= fun _ -> Some (|k, v|)
+  
+let lens_case (p:(k:'a -> pcm ('b k))) (k:'a): lens (refine_t (case_refinement_f p k)) ('b k) = {
+  get = lens_case_get p k;
+  put = lens_case_put p k;
+  get_put = (fun s v -> ());
+  put_get = (fun s -> ());
+  put_put = (fun s v w -> ());
+}
+
+(** lens_case is a pcm_lens *)
+let case (p:(k:'a -> refined_one_pcm ('b k))) (k:'a)
+: pcm_lens (refined_pcm (case_refinement p k)) (p k) = {
+  l = lens_case p k;
+  get_morphism = {f_refine = (fun _ -> ()); f_one = (fun _ -> ()); f_op = (fun _ _ -> ())};
+  put_morphism = {f_refine = (fun _ -> ()); f_one = (fun _ -> ()); f_op = (fun _ _ -> ())};
+}
 
 (** Refining a pcm_lens *)
 
@@ -324,7 +420,7 @@ val ref_refine
 
 module A = Steel.Effect.Atomic
 
-val ref_focus (r: ref 'a 'b) (q: refined_one_pcm 'c) (l: pcm_lens r.q q): ref 'a 'c
+let ref_focus (r: ref 'a 'b) (q: refined_one_pcm 'c) (l: pcm_lens r.q q): ref 'a 'c = {p = r.p; re = r.re; u = r.u; q = q; pl = pcm_lens_comp r.pl l; r = r.r}
 
 val split (r: ref 'a 'c) (xy x y: Ghost.erased 'c)
 : Steel unit
