pulse/examples/steel/PointStruct.fsti
@@ -1,0 +1,92 @@
+module PointStruct
+
+open Aggregates
+open AggregateRef
+open PCM.POD
+open FStar.PCM
+//open FStar.FunctionalExtensionality
+open Steel.Effect
+//module A = Steel.Effect.Atomic
+
+/// Suppose we have the following struct representing 2d points:
+///   struct point { int x, y; };
+///
+/// Carrier of PCM for struct point:
+
+val point : Type0
+
+/// PCM for struct point:
+
+val point_pcm : pcm point
+
+/// (mk_point x y) represents (struct point){.x = x, .y = y}
+
+val mk_point (x y: pod int): point
+
+/// PCM lenses for the fields of a point
+
+val _x : pcm_lens point_pcm (pod_pcm int)
+val _y : pcm_lens point_pcm (pod_pcm int)
+
+(*
+/// Laws relating _x, _y, and mk_point
+
+val point_put_x (x' x y: pod int)
+: Lemma (put _x x' (mk_point x y) == mk_point x' y)
+  [SMTPat (put _x x' (mk_point x y))]
+
+val point_get_x (x y: pod int)
+: Lemma (get _x (mk_point x y) == x)
+  [SMTPat (get _x (mk_point x y))]
+
+val point_put_y (y' x y: pod int)
+: Lemma (put _y y' (mk_point x y) == mk_point x y')
+  [SMTPat (put _y y' (mk_point x y))]
+
+val point_get_y (x y: pod int)
+: Lemma (get _y (mk_point x y) == y)
+  [SMTPat (get _y (mk_point x y))]
+
+/// Laws relating mk_point to PCM operations
+
+val point_one : squash (one point_pcm == mk_point none none)
+
+val point_op (x y x' y': pod int)
+: Lemma
+    (requires composable (pod_pcm int) x x' /\ composable (pod_pcm int) y y')
+    (ensures composable point_pcm (mk_point x y) (mk_point x' y') /\
+     op point_pcm (mk_point x y) (mk_point x' y') == mk_point (op (pod_pcm int) x x') (op (pod_pcm int) y y'))
+  [SMTPat (op point_pcm (mk_point x y) (mk_point x' y'))]
+*)
+
+/// Taking pointers to the x and y fields of a point
+
+val addr_of_x (p: ref 'a point{p.q == point_pcm}) (x y: Ghost.erased (pod int))
+: SteelT (q:ref 'a (pod int){q == ref_focus p (pod_pcm int) _x})
+    (p `pts_to` mk_point x y)
+    (fun q ->
+       (p `pts_to` mk_point none y) `star`
+       (q `pts_to` x))
+
+val un_addr_of_x
+  (p: ref 'a point{p.q == point_pcm})
+  (q: ref 'a (pod int){q == ref_focus p (pod_pcm int) _x})
+  (x y: Ghost.erased (pod int))
+: SteelT unit
+    ((p `pts_to` mk_point none y) `star` (q `pts_to` x))
+    (fun q -> p `pts_to` mk_point x y)
+
+val addr_of_y (p: ref 'a point{p.q == point_pcm}) (x y: Ghost.erased (pod int))
+: SteelT (q:ref 'a (pod int){q == ref_focus p (pod_pcm int) _y})
+    (p `pts_to` mk_point x y)
+    (fun q ->
+       (p `pts_to` mk_point x none) `star`
+       (q `pts_to` y))
+
+val un_addr_of_y
+  (p: ref 'a point{p.q == point_pcm})
+  (q: ref 'a (pod int){q == ref_focus p (pod_pcm int) _y})
+  (x y: Ghost.erased (pod int))
+: SteelT unit
+    ((p `pts_to` mk_point x none) `star` (q `pts_to` y))
+    (fun q -> p `pts_to` mk_point x y)
